helping/HelpingOff.v
@@ -8,7 +8,7 @@ Module HelpingOff. Section HelpingOff.
   Context {jobID retID : Type}.
   Context (jobcode : jobID → itree Helping.pureE retID).
 
-  Definition scopes := [mn].
+  Definition scopes : gmultiset string := {[+mn+]}.
 
   Definition run : Any.t → itree crisE Any.t :=
     λ arg,
@@ -19,17 +19,17 @@ Module HelpingOff. Section HelpingOff.
   Definition help : Any.t → itree crisE Any.t :=
     λ _, 𝒴;;; Ret ()↑.
       
-  Definition fnsems : alist (option string) (fnsem_type (option fspec * fbody)) :=
-    [(Some (Helping.run mn),  (true, wmask_all, scopes, (None, run)));
-     (Some (Helping.help mn), (true, wmask_all, scopes, (None, help)))].
+  Definition fnsems : gmap (option string) (option (emask * (option fspec * fbody))) :=
+    {[Some (Helping.run mn) := Some (msk_scp scopes msk_true, (Some fspec_trivial, run));
+      Some (Helping.help mn) := Some (msk_scp scopes msk_true, (Some fspec_trivial, help))]}.
 
   Program Definition Mod : SMod.t := {|
     SMod.scopes := scopes;
     SMod.fnsems := fnsems;
-    SMod.initial_st := [];
+    SMod.initial_st := ∅;
   |}.
-  Solve All Obligations with prove_scope.
-  Next Obligation. prove_nodup. Qed.
+  Solve All Obligations with try done.
+  Next Obligation. rewrite ?omap_insert omap_empty /=. mod_tac scope_solver. Qed.
 
-  Definition t sp := Seal.sealing CRIS (SMod.to_mod sp Mod).  
+  Definition t sp := SMod.to_mod sp Mod.
 End HelpingOff. End HelpingOff.
