helping/HelpingOn.v
@@ -3,7 +3,7 @@ From iris.algebra Require Import gmap_view.
 From CRIS.helping Require Import Header.
 From stdpp Require Import fin_sets.
 
-Section HoareCall.
+(* Section HoareCall.
   Context `{!crisG Γ Σ α β τ _S _I, !concG}.
 
   Definition fspec_option_meta (fspo : option fspec) : Type :=
@@ -15,7 +15,7 @@ Section HoareCall.
   Definition HoareCall_prologue fspo varg : itree crisE (fspec_option_meta fspo * Any.t) :=
     Seal.sealing "Help"
     (match fspo as fspo return itree crisE (fspec_option_meta fspo * Any.t) with
-    | Some (@fspec_call _ meta pre post) =>
+    | Some (@fspec_mk _ meta pre post) =>
         x <- trigger (Choose meta);;
         arg <- trigger (Choose Any.t);;
         trigger (Guarantee (pre x varg arg));;;
@@ -75,7 +75,7 @@ Section HoareCall.
     | Some _ => λ _, triggerNB
     | None => λ _, Ret vret
     end) x.
-End HoareCall.
+End HoareCall. *)
 
 (* Helping module *)
 Module HelpingOn. Section HelpingOn.
@@ -84,8 +84,8 @@ Module HelpingOn. Section HelpingOn.
   Context (mn : string).
   Context (jobcode : jobID → itree Helping.pureE retID).
 
-  Definition scopes := [mn].
-  Definition v_reqs := mn ↯ "reqs".
+  Definition scopes : gmultiset string := {[+mn+]}.
+  Definition v_reqs : key := mn ↯ "reqs".
 
   Definition try_run (tid : nat) : itree crisE retID :=
     'reqs : gmap nat (option retID * jobID) <- cgetU v_reqs;;
@@ -106,47 +106,48 @@ Module HelpingOn. Section HelpingOn.
       cput v_reqs (<[tid := (None, jid)]> reqs);;;
       𝒴;;; r <- try_run tid;; 𝒴;;; Ret (r↑).
 
-  Definition help (sp : sp_type) : Any.t → itree crisE Any.t :=
+  Definition help (sp : specmap) : Any.t → itree crisE Any.t :=
     λ _,
       tid <- trigger (Choose nat);;
-      xarg <- HoareCall_prologue (sp SchHdr.yield) (() ↑);;
-      x <- HoareFun_prologue (sp SchHdr.yield) (() ↑);;
+      (* xarg <- HoareCall_prologue (sp SchHdr.yield) (() ↑);;
+      x <- HoareFun_prologue (sp SchHdr.yield) (() ↑);; *)
       try_run tid;;;
-      HoareFun_epilogue (sp SchHdr.yield) x.1 (() ↑);;;
-      HoareCall_epilogue (sp SchHdr.yield) xarg.1 (() ↑);;;
+      (* HoareFun_epilogue (sp SchHdr.yield) x.1 (() ↑);;;
+      HoareCall_epilogue (sp SchHdr.yield) xarg.1 (() ↑);;; *)
       Ret ()↑.
 
-  Definition fnsems (sp : sp_type) : alist (option string) (fnsem_type (option fspec * fbody)) :=
-    [(Some (Helping.run mn),  (true, wmask_all, scopes, (None, run)));
-     (Some (Helping.help mn), (true, wmask_all, scopes, (None, help sp)))].
+  Definition fnsems (sp : specmap) : gmap (option string) (option (emask * (option fspec * fbody))) :=
+    {[Some (Helping.run mn) := Some (msk_scp scopes msk_true, (Some fspec_trivial, run));
+      Some (Helping.help mn) := Some (msk_scp scopes msk_true, (Some fspec_trivial, help sp))]}.
 
-  Program Definition Mod (sp : sp_type) : SMod.t := {|
+  Program Definition Mod (sp : specmap) : SMod.t := {|
     SMod.scopes := scopes;
     SMod.fnsems := fnsems sp;
-    SMod.initial_st := [(v_reqs, (∅ : gmap nat (option retID * jobID))↑)];
+    SMod.initial_st := {[v_reqs := Some (∅ : gmap nat (option retID * jobID))↑]};
   |}.
-  Solve All Obligations with prove_scope.
-  Next Obligation. prove_nodup. Qed.
+  Next Obligation. i; rewrite ?omap_insert omap_empty /=; mod_tac scope_solver. Qed.
+  Next Obligation. set_solver. Qed.
+  Next Obligation. i; mod_tac scope_solver. Qed.
 
-  Definition t sp : Mod.t := Seal.sealing CRIS (SMod.to_mod sp (Mod sp)).
+  Definition t sp : Mod.t := SMod.to_mod sp (Mod sp).
 End HelpingOn. End HelpingOn.
 
 Module HelpingDummy. Section HelpingDummy.
   Context `{!crisG Γ Σ α β τ _S _I, !concG}.
   Context (mn : string).
-  Definition scopes := [mn].
+  Definition scopes : gmultiset string := {[+mn+]}.
 
-  Definition fnsems : alist (option string) (fnsem_type (option fspec * fbody)) :=
-    [(Some (Helping.run mn),  (true, wmask_all, scopes, (None, λ _, triggerNB)));
-     (Some (Helping.help mn), (true, wmask_all, scopes, (None, λ _, triggerNB)))].
+  Definition fnsems : gmap (option string) (option (emask * (option fspec * fbody))) :=
+    {[Some (Helping.run mn) := Some (msk_scp scopes msk_true, (None, λ _, triggerNB));
+      Some (Helping.help mn) := Some (msk_scp scopes msk_true, (None, λ _, triggerNB))]}.
 
   Program Definition Mod : SMod.t := {|
     SMod.scopes := scopes;
     SMod.fnsems := fnsems;
-    SMod.initial_st := [];
+    SMod.initial_st := ∅;
   |}.
-  Solve All Obligations with prove_scope.
-  Next Obligation. prove_nodup. Qed.
+  Solve All Obligations with try done.
+  Next Obligation. rewrite ?omap_insert omap_empty /=; mod_tac scope_solver. Qed.
 
-  Definition t : Mod.t := Seal.sealing CRIS (SMod.to_mod sp_none Mod).
+  Definition t : Mod.t := SMod.to_mod ∅ Mod.
 End HelpingDummy. End HelpingDummy.
