scheduler/SchI.v
@@ -6,7 +6,7 @@ Definition thpool : Type := list (nat * option SAny.t).
 Module SchI. Section SchI.
   Context `{!crisG Γ Σ α β τ _S _I, !concG}.
 
-  Definition scp : gmultiset string := {[+"sch"+]}.
+  Definition scopes : gmultiset string := {[+"sch"+]}.
   Definition v_ths : key := "sch" ↯ "ths".
   Definition v_tid : key := "sch" ↯ "tid".
 
@@ -62,14 +62,14 @@ Module SchI. Section SchI.
     λ _, cgetU v_tid.
 
   Definition fnsems : gmap (option string) (option (emask * (option fspec * fbody))) :=
-    {[Some SchHdr._spawn := Some (msk_real (msk_scp scp msk_true), (None, cfunU inner_spawn));
-      Some SchHdr.spawn := Some (msk_real (msk_scp scp msk_true), (None, cfunU spawn));
-      Some SchHdr.yield := Some (msk_real (msk_scp scp msk_true), (None, cfunU yield));
-      Some SchHdr.join := Some (msk_real (msk_scp scp msk_true), (None, cfunU join));
-      Some SchHdr.get_tid := Some (msk_real (msk_scp scp msk_true), (None, cfunU get_tid))]}.
+    {[Some SchHdr._spawn := Some (msk_real (msk_scp scopes msk_true), (None, cfunU inner_spawn));
+      Some SchHdr.spawn := Some (msk_real (msk_scp scopes msk_true), (None, cfunU spawn));
+      Some SchHdr.yield := Some (msk_real (msk_scp scopes msk_true), (None, cfunU yield));
+      Some SchHdr.join := Some (msk_real (msk_scp scopes msk_true), (None, cfunU join));
+      Some SchHdr.get_tid := Some (msk_real (msk_scp scopes msk_true), (None, cfunU get_tid))]}.
 
   Program Definition smod : SMod.t := {|
-    SMod.scopes := scp;
+    SMod.scopes := scopes;
     SMod.fnsems := fnsems;
     SMod.initial_st := {[v_ths:=Some ([(0, None)] : thpool)↑; v_tid := Some 0↑]};
   |}.
